Tests/UIDEquivSpec.lean
@@ -15,41 +15,46 @@ def group : UIDEquiv Nat Nat where
     intro id
     rfl
 
-@[reducible] def boolMetadata : Aux group (λ _value => Bool) where
-  Evidence := λ _id => Bool
+@[reducible] def eqOneMetadata : Aux group (λ value => value = 1) where
+  Ev := λ id => group.inv id = 1
   lookup := λ _id => none
   getEv := λ bundle => bundle.snd
   invEv := λ id2 => id2.snd
 
 @[reducible] def unitMetadata : Aux group (λ _value => Unit) where
-  Evidence := λ _id => Unit
+  Ev := λ _id => True
   lookup := λ _id => none
-  getEv := λ bundle => bundle.snd
-  invEv := λ id2 => id2.snd
+  getEv := λ _bundle => True.intro
+  invEv := λ _id2 => ()
 
 section getUID
 
 example :
-    boolMetadata.Evidence (group.getUID 1) :=
-  boolMetadata.getEv ⟨1, true⟩
+    eqOneMetadata.Ev (group.getUID 1) :=
+  eqOneMetadata.getEv ⟨1, rfl⟩
 
 example :
-    boolMetadata.Evidence (group.getUID 1) ×
-      unitMetadata.Evidence (group.getUID 1) :=
-  ⟨boolMetadata.getEv ⟨1, true⟩,
+    eqOneMetadata.Ev (group.getUID 1) ∧
+      unitMetadata.Ev (group.getUID 1) :=
+  ⟨eqOneMetadata.getEv ⟨1, rfl⟩,
     unitMetadata.getEv ⟨1, ()⟩⟩
 
 example :
     group.inv (group.getUID 1) = 1 := by
-  exact boolMetadata.leftInvValue ⟨1, true⟩
+  exact eqOneMetadata.leftInvValue ⟨1, rfl⟩
 
 example :
-    boolMetadata.invEv
-      ⟨group.getUID 1, boolMetadata.getEv ⟨1, true⟩⟩ = true := by
+    eqOneMetadata.invEv
+      ⟨group.getUID 1, eqOneMetadata.getEv ⟨1, rfl⟩⟩ = rfl := by
   rfl
 
 example :
-    boolMetadata.lookup (group.getUID 1) = none := by
+    unitMetadata.invEv
+      ⟨group.getUID 1, unitMetadata.getEv ⟨1, ()⟩⟩ = () := by
+  rfl
+
+example :
+    eqOneMetadata.lookup (group.getUID 1) = none := by
   rfl
 
 end getUID
